Add lemmas from walkup.v to my theory

Walkup.thy
@@ -91,9 +91,11 @@ proof
     show "inj_on (skip_edge z H) (A - {z})"
       by (smt (z3) apply_inj_eq_iff faceK inj_on_def skip_edge_def)
     show "\<And>x. x \<in> (A - {z}) \<Longrightarrow> skip_edge z H x \<in> (A - {z})"
-      by (smt (z3) Diff_iff \<open>A = darts H\<close> apply_inj_eq_iff empty_iff faceK perm_edge perm_face insert_iff permutes_in_image skip_edge_def)
+      by (smt (z3) Diff_iff \<open>A = darts H\<close> apply_inj_eq_iff empty_iff faceK
+          perm_edge perm_face insert_iff permutes_in_image skip_edge_def)
     show "\<And>x. x \<notin> (A - {z}) \<Longrightarrow> skip_edge z H x = x"
-      by (smt (z3) Diff_empty Diff_insert0 Permutations.permutes_not_in \<open>A = darts H\<close> perm_edge perm_face insert_Diff insert_iff skip_edge_def)
+      by (smt (z3) Diff_empty Diff_insert0 Permutations.permutes_not_in \<open>A = darts H\<close>
+          perm_edge perm_face insert_Diff insert_iff skip_edge_def)
   qed
 qed
 
@@ -115,49 +117,28 @@ next
   show "\<forall>y. \<exists>!x. skip_edge z H x = y"
     by (metis skip_edge_Perm UNIV_I bij_apply bij_imp_permutes permutes_univ)
 qed
-end
 
-locale not_degenerate_walkup = hypermap +
-  fixes z
-  assumes z_dart: "z \<in> darts H"
-      and z_not_glink: "\<not>z\<rightarrow>\<^bsub>glink H\<^esub>z"
-begin
+lemma skip_edgeK: "skip_edge z H (skip z (node H) (skip z (face H) x)) = x"
+  by (smt (z3) edgeK faceK nodeK skip_def skip_edge_def)
 
-lemma skip_edge_edge: "skip_edge z H (node H (face H z)) = (edge H (node H z))"
-  unfolding skip_edge_def
-  by (metis Gr_eq cedge_def cface_def edgeK glink_def not_degenerate_walkup.axioms(2) 
-      not_degenerate_walkup_axioms not_degenerate_walkup_axioms_def pair_union_arcs_disj)
+lemma skip_edge_noteq_z: "x \<noteq> z \<Longrightarrow> skip_edge z H x \<noteq> z"
+  by (metis apply_inj_eq_iff skip_edge_Perm skip_edge_id)
 
-lemma skip_edge_node: "skip_edge z H (node H z) = (edge H z)"
-  unfolding skip_edge_def
-  by (metis Gr_eq cnode_def edgeK faceK glink_def not_degenerate_walkup.axioms(2) 
-      not_degenerate_walkup_axioms not_degenerate_walkup_axioms_def pair_union_arcs_disj
-      skip_edge_def skip_edge_edge)
-
-lemma skip_edge_invariant:
-  fixes x
-  assumes "x \<noteq> z" "face H (edge H x) \<noteq> z" "edge H x \<noteq> z"
-  shows "skip_edge z H x = edge H x"
-  unfolding skip_edge_def using assms by auto
-end
-
-text "Degenerate case for walkup where one of the permutations is an identity on z"
-lemma (in hypermap) glink_skip_edge:
-  assumes "z\<rightarrow>\<^bsub>glink H\<^esub>z"
-  shows "skip_edge z H = skip z (edge H)"
+lemma (in hypermap) glink_skip_edge: "z\<rightarrow>\<^bsub>glink H\<^esub>z \<Longrightarrow> skip_edge z H = skip z (edge H)"
 proof
-  fix x
-  from assms have z_eq: "z = edge H z \<or> z = node H z \<or> z = face H z"
+  fix x assume *: "z\<rightarrow>\<^bsub>glink H\<^esub>z"
+  then have z_eq: "z = edge H z \<or> z = node H z \<or> z = face H z"
     unfolding glink_def cedge_def cnode_def cface_def by (metis Gr_eq pair_union_arcs_disj)
   have "z = edge H z \<Longrightarrow> skip_edge z H x = skip z (edge H) x"
     by (simp add: skip_def skip_edge_def)
   also have "z = node H z \<Longrightarrow> skip_edge z H x = skip z (edge H) x"
-    unfolding skip_edge_def skip_def using assms nodeK by fastforce
+    unfolding skip_edge_def skip_def using * nodeK by fastforce
   moreover have "z = face H z \<Longrightarrow> skip_edge z H x = skip z (edge H) x"
-    unfolding skip_edge_def skip_def using assms faceK by auto
+    unfolding skip_edge_def skip_def using * faceK by auto
   ultimately show "skip_edge z H x = skip z (edge H) x"
     using z_eq by blast
 qed
+end
 
 section \<open>WalkupE\<close>
 
@@ -168,33 +149,75 @@ definition walkupE :: "'a pre_hypermap \<Rightarrow> 'a \<Rightarrow> 'a pre_hyp
    node = skip_perm z (node h),
    face = skip_perm z (face h)\<rparr>"
 
-theorem (in hypermap) hypermap_walkupE:
-  shows "hypermap (walkupE H z)" (is "hypermap ?E")
+locale walkup = hypermap +
+  fixes z
+  assumes z_dart: "z \<in> darts H"
+begin
+  definition "H' \<equiv> walkupE H z"
+
+lemma walkup_edge: "edge H' = Perm (skip_edge z H)"
+  by (simp add: H'_def walkupE_def)
+
+lemma walkup_node: "node H' = skip_perm z (node H)"
+  by (simp add: H'_def walkupE_def)
+
+lemma walkup_face: "face H' = skip_perm z (face H)"
+  by (simp add: H'_def walkupE_def)
+end
+
+locale not_degenerate_walkup = walkup +
+  fixes u v
+  assumes z_not_glink: "\<not>z\<rightarrow>\<^bsub>glink H\<^esub>z"
+      and dart_u: "u \<in> darts H'"
+      and dart_v: "v \<in> darts H'"
+begin
+
+lemma u_noteq_z: "u \<noteq> z"
+  by (metis dart_u DiffE H'_def insert_iff pre_hypermap.select_convs(1) walkupE_def)
+
+lemma v_noteq_z: "v \<noteq> z"
+  by (metis dart_v DiffE H'_def insert_iff pre_hypermap.select_convs(1) walkupE_def)
+
+lemma skip_edge_edge: "skip_edge z H (node H (face H z)) = (edge H (node H z))"
+  unfolding skip_edge_def
+  by (metis Gr_eq cedge_def cface_def edgeK glink_def pair_union_arcs_disj z_dart z_not_glink)
+
+lemma skip_edge_node: "skip_edge z H (node H z) = (edge H z)"
+  unfolding skip_edge_def
+  by (smt (z3) Gr_eq apply_perm_image cnode_def darts_face edgeK glink_def imageE
+      pair_union_arcs_disj skip_edge_def skip_edge_edge z_dart z_not_glink)
+
+lemma skip_edge_invariant:
+  fixes x
+  assumes "x \<noteq> z" "face H (edge H x) \<noteq> z" "edge H x \<noteq> z"
+  shows "skip_edge z H x = edge H x"
+  unfolding skip_edge_def using assms by auto
+
+lemma walkup_darts_subset: "darts H' \<subseteq> darts H"
+  unfolding H'_def walkupE_def by simp
+end
+
+context walkup 
+begin
+theorem hypermap_walkupE:
+  shows "hypermap H'"
 proof
   have "finite (darts H)" by (rule finite_darts)
-  also have "(darts ?E) = (darts H) - {z}"
-    by (simp add: walkupE_def)
-  ultimately show "finite (darts ?E)" by auto
-  show "edge (walkupE H z) permutes darts (walkupE H z)"
-    by (simp add: finite_darts hypermap_axioms permutes_perm skip_edge_permutes walkupE_def)
-  show "(node (walkupE H z)) permutes darts (walkupE H z)"
-    by (simp add: walkupE_def apply_skip_perm perm_node skip_permutes)
-  show "(face (walkupE H z)) permutes darts (walkupE H z)"
-    by (simp add: walkupE_def apply_skip_perm perm_face skip_permutes)
-next
-  fix x have "skip_edge z H (skip z (node H) (skip z (face H) x)) = x"
-  proof (cases "x = z")
-    case True
-    then show ?thesis
-      by simp
-  next
-    case False
-    then show ?thesis
-      by (smt (z3) apply_inj_eq_iff faceK skip_def skip_edge_def)
-  qed
-  then show "(edge (walkupE H z)) \<langle>$\<rangle> (node (walkupE H z)) \<langle>$\<rangle> (face (walkupE H z)) \<langle>$\<rangle> x = x"
-    by (simp add: apply_skip_perm skip_edge_Perm walkupE_def)
+  also have "(darts H') = (darts H) - {z}"
+    by (simp add: H'_def walkupE_def)
+  ultimately show "finite (darts H')" by auto
+  show "edge H' permutes darts (H')"
+    by (simp add: H'_def finite_darts hypermap_axioms permutes_perm skip_edge_permutes walkupE_def)
+  show "(node (H')) permutes darts (H')"
+    by (simp add: H'_def walkupE_def apply_skip_perm perm_node skip_permutes)
+  show "(face (H')) permutes darts (H')"
+    by (simp add: H'_def walkupE_def apply_skip_perm perm_face skip_permutes)
+  fix x show "(edge (H')) \<langle>$\<rangle> (node (H')) \<langle>$\<rangle> (face (H')) \<langle>$\<rangle> x = x"
+    by (simp add: H'_def skip_edgeK apply_skip_perm skip_edge_Perm walkupE_def)
 qed
+
+lemma card_darts_walkup: "card (darts H') = card (darts H) - 1"
+  by (simp add: H'_def finite_darts walkupE_def z_dart)
 
 text \<open>(From fourcolour.walkup.v)
  cross_edge z <=> z and node z are on the same edge cycle. This edge cycle 
@@ -204,40 +227,345 @@ text \<open>(From fourcolour.walkup.v)
                  planarity condition are invariant.
 \<close>
 
-definition cross_edge where
-"cross_edge h z \<equiv> z\<rightarrow>\<^sup>*\<^bsub>cedge h\<^esub>node h z"
+definition "cross_edge \<equiv> z\<rightarrow>\<^sup>*\<^bsub>cedge H\<^esub>node H z"
 
-lemma (in hypermap) cross_edge_path_edge:
-  "cross_edge H z \<longleftrightarrow> edge H z\<rightarrow>\<^sup>*\<^bsub>cedge H\<^esub>node H z" (is "?L = ?R")
+lemma cross_edge_path_edge:
+  "cross_edge \<longleftrightarrow> edge H z\<rightarrow>\<^sup>*\<^bsub>cedge H\<^esub>node H z" (is "?L = ?R")
 proof
   assume ?L show ?R
   proof (rule wf_digraph.reachable_trans)
     show "wf_digraph (cedge H)"
       by (simp add: wf_cedge wf_digraph_wp_iff)
     then show "(edge H) \<langle>$\<rangle> z \<rightarrow>\<^sup>*\<^bsub>with_proj (cedge H)\<^esub> z"
-      by (metis (no_types, lifting) \<open>cross_edge H z\<close> Gr_eq Permutations.permutes_not_in cedge_def
-          hypermap.cedge_reachable_sym cross_edge_def hypermap_axioms perm_edge
-          reach_sym_arc wf_digraph.reachable_in_verts(1) wf_digraph.reachable_refl)
+      by (metis Gr_eq cedge_connect_sym cedge_def wf_digraph.reach_sym_arc z_dart)
     show "z \<rightarrow>\<^sup>*\<^bsub>with_proj (cedge H)\<^esub> (node H) \<langle>$\<rangle> z"
-      using \<open>cross_edge H z\<close> unfolding cross_edge_def by simp
+      using \<open>cross_edge\<close> unfolding cross_edge_def by simp
   qed
 next
-  assume ?R show ?L
-    by (metis Gr_eq Permutations.permutes_not_in cedge_def cross_edge_def
-        \<open>(edge H) \<langle>$\<rangle> z \<rightarrow>\<^sup>*\<^bsub>with_proj (cedge H)\<^esub> (node H) \<langle>$\<rangle> z\<close> perm_edge wf_cedge 
-        wf_digraph.adj_reachable_trans wf_digraph_wp_iff)
+  assume ?R then show ?L
+    by (metis Gr_eq cedge_def cross_edge_def wf_cedge wf_digraph.adj_reachable_trans 
+        wf_digraph_wp_iff z_dart)
 qed
 
-locale degenerate_walkup = hypermap +
-  fixes z
+interpretation clink: fin_digraph "clink H"
+  by (simp add: finite_clink)
+
+definition z_comp where
+"z_comp \<equiv> (clink H') \<restriction> (clink.scc_of z - {z})"
+
+lemma wf_z_comp: "wf_digraph z_comp"
+   by (simp add: fin_digraph.axioms(1) hypermap.finite_clink hypermap_walkupE 
+        wf_digraph.wellformed_induce_subgraph z_comp_def)
+
+interpretation z_comp: fin_digraph z_comp
+proof intro_locales
+  show "wf_digraph z_comp" using wf_z_comp .
+  have "finite (verts z_comp)"
+    by (metis clink.finite_verts clink.scc_of_empty_conv clink.scc_of_in_sccs_verts 
+        clink.sccs_verts_subsets finite_Diff finite_subset induce_subgraph_verts 
+        infinite_imp_nonempty z_comp_def)
+  also {
+    have "clink.scc_of z \<subseteq> verts (clink H)"
+      using clink.scc_of_empty_conv clink.scc_of_in_sccs_verts clink.sccs_verts_subsets by blast
+    then have "clink.scc_of z - {z} \<subseteq> verts (clink H)"
+      using calculation by blast
+    then have "arcs z_comp \<subseteq> arcs (clink H')"
+      by (simp add: z_comp_def)
+    then have "finite (arcs z_comp)"
+      by (meson fin_digraph.finite_arcs finite_subset hypermap.finite_clink hypermap_walkupE)
+  }
+  ultimately show "fin_digraph_axioms z_comp"
+    using fin_digraph_axioms.intro by blast
+qed
+
+definition z_barb where
+"z_barb \<equiv> clink.scc_of z = {z}"
+
+lemma z_barb_z: "z_barb = (edge H z = z \<and> node H z = z \<and> face H z = z)"
+proof
+  assume *: "z_barb"
+  then show "edge H z = z \<and> node H z = z \<and> face H z = z"
+    by (smt (verit) DiffD2 apply_inj_eq_iff clink.in_sccs_verts_conv_reachable
+        clink.scc_of_in_sccs_verts clinkN clink_connect_sym fst_conv hypermap.clinkF hypermap_axioms
+        insert_Diff insert_iff nodeK pair_wf_digraph.arc_fst_in_verts wf_clink
+        wf_digraph.reachable_adjI wf_digraph_wp_iff with_proj_simps(1) with_proj_simps(3)
+        z_barb_def z_dart clink.wf_digraph_axioms wf_digraph.reach_sym_arc)
+next
+  assume assms: "(edge H z = z \<and> node H z = z \<and> face H z = z)"
+  then have "node H z = z \<and> face H z = z"
+    by simp
+  {
+    fix x assume *: "x \<in> clink.scc_of z" "x \<noteq> z"
+    then have "False" 
+    proof -
+      have "x\<rightarrow>\<^sup>*\<^bsub>clink H\<^esub>z"
+        using *(1) clink.scc_of_def by blast
+      then obtain y where "y \<noteq> z \<and> y\<rightarrow>\<^bsub>clink H\<^esub>z"
+        by (smt (verit) "*"(2) clink.awalk_ends clink.reachable_awalk wf_clink 
+              wf_digraph.converse_reachable_induct wf_digraph_wp_iff)
+      also have "\<And>u. u \<rightarrow>\<^bsub>clink H\<^esub>z \<Longrightarrow> u = z"
+        unfolding clink_def
+        by (metis Gr_eq assms apply_inj_eq_iff cface_def cnode_def converse_iff
+            pair_pre_digraph.simps(2) pair_union_arcs_disj reverse_def with_proj_simps(3))
+      ultimately show ?thesis
+        by auto
+    qed
+    then have "x \<in> clink.scc_of z \<Longrightarrow> x = z"
+      by blast
+  }
+  then show "z_barb"
+    using clink.wf_digraph_axioms clinkF pre_digraph.scc_of_def wf_digraph.adj_in_verts(1)
+      z_barb_def z_dart by fastforce
+qed
+                                                    
+lemma z_barb_comp: "z_barb = (pre_digraph.sccs z_comp = {})"
+proof
+  assume z_barb
+  then have "verts z_comp = {}"
+    unfolding z_barb_def z_comp_def by simp
+  moreover have "arcs z_comp = {}"
+    by (metis wf_z_comp calculation ex_in_conv wf_digraph.wellformed(2))
+  ultimately show "pre_digraph.sccs z_comp = {}"
+    by (metis antisym_conv bot.extremum equals0I pre_digraph.in_sccsE
+        pre_digraph.induced_subgraph_altdef strongly_connected_def subgraph_def)
+next
+  assume "pre_digraph.sccs z_comp = {}"
+  then have "verts z_comp = {}"
+    by (metis empty_iff equals0I wf_digraph.in_verts_sccsD_sccs 
+        wf_digraph.scc_of_in_sccs_verts wf_z_comp) 
+  then have "clink.scc_of z - {z} = {}"
+    using z_comp_def by force 
+  then have "clink.scc_of z = {z}"
+    by (metis clink.adj_in_verts(2) clink.in_scc_of_self
+        clinkN insert_Diff walkup.z_dart walkup_axioms)
+  then show z_barb
+    unfolding H'_def z_comp_def z_barb_def by blast
+qed
+
+
+definition "disconnected \<equiv> card (pre_digraph.sccs z_comp) > 1"
+
+lemma disconnected_not_glink: "disconnected \<Longrightarrow> \<not> z\<rightarrow>\<^bsub>glink H\<^esub>z"
+proof
+  assume *: disconnected "z\<rightarrow>\<^bsub>glink H\<^esub>z"
+  then have "\<not>z_barb"
+    using disconnected_def z_barb_comp by force
+  have "strongly_connected z_comp"
+  proof
+    show "verts z_comp \<noteq> {}"
+      using \<open>\<not> z_barb\<close> z_barb_comp z_comp.sccs_conv_sccs_verts z_comp.sccs_verts_conv_scc_of
+      by force
+    show "u \<in> verts z_comp \<Longrightarrow> v \<in> verts z_comp \<Longrightarrow> u \<rightarrow>\<^sup>*\<^bsub>z_comp\<^esub> v" for u v
+      sorry
+  qed
+  then have "card (pre_digraph.sccs z_comp) = 1"
+    using wf_digraph.card_sccs_connected wf_z_comp by blast
+  then show False
+    using *(1) disconnected_def by linarith
+qed
+
+lemma disconnected_cross_edge: "disconnected \<Longrightarrow> cross_edge"
+  sorry
+
+corollary not_cross_connected: "\<not> cross_edge \<Longrightarrow> \<not> disconnected"
+  using disconnected_cross_edge by auto
+
+lemma (in not_degenerate_walkup) clink_at_G': "u \<rightarrow>\<^bsub>clink H\<^esub>v \<Longrightarrow> u\<rightarrow>\<^bsub>clink H'\<^esub>v"
+proof -
+  assume "u \<rightarrow>\<^bsub>clink H\<^esub>v"
+  then have "(v\<rightarrow>\<^bsub>cnode H\<^esub> u \<or> u \<rightarrow>\<^bsub>cface H\<^esub> v)" (is "?N \<or> ?F")
+    by (metis clink_def converse_iff pair_pre_digraph.simps(2) pair_union_arcs_disj
+        reverse_def with_proj_simps(3))
+  also have "v\<rightarrow>\<^bsub>cnode H\<^esub> u \<Longrightarrow> v\<rightarrow>\<^bsub>cnode H'\<^esub> u"
+    by (metis Gr_eq H'_def apply_skip_perm cnode_def dart_v pre_hypermap.select_convs(3)
+        skip_def u_noteq_z v_noteq_z walkupE_def)
+  moreover have "u \<rightarrow>\<^bsub>cface H\<^esub> v \<Longrightarrow> u \<rightarrow>\<^bsub>cface H'\<^esub> v"
+    by (metis Gr_eq H'_def apply_skip_perm cface_def dart_u pre_hypermap.select_convs(4)
+        skip_def u_noteq_z v_noteq_z walkupE_def)
+  ultimately show ?thesis
+    by (meson dart_u dart_v hypermap.clinkP hypermap_walkupE)
+qed
+
+lemma (in not_degenerate_walkup) clink_at_H:
+  shows "u \<rightarrow>\<^sup>*\<^bsub>clink H'\<^esub>v \<Longrightarrow> u\<rightarrow>\<^sup>*\<^bsub>clink H\<^esub>v"
+proof -
+  interpret clink': wf_digraph "clink H'"
+    using hypermap.wf_clink hypermap_walkupE wf_digraph_wp_iff by blast
+  interpret clink: wf_digraph "clink H"
+    by (simp add: wf_clink wf_digraph_wp_iff)
+  assume "u \<rightarrow>\<^sup>*\<^bsub>clink H'\<^esub>v"
+  then obtain p' where "clink'.awalk u p' v"
+    using clink'.reachable_awalk by blast
+  then have "\<exists>p. clink.awalk u p v"
+  proof (induct rule: clink'.awalk_induct_raw)
+    case Base
+    then show ?case
+      by (simp add: \<open>clink'.awalk u p' v\<close>)
+  next
+    case (Cons w)
+    then have "w \<in> darts H'"
+      unfolding clink_def cface_def cnode_def by (simp add: reverse_def)
+    then have "w \<in> verts (clink H)"
+      unfolding clink_def cface_def cnode_def reverse_def 
+      using walkup_darts_subset by auto
+    then have "clink.awalk w [] w"
+      by (simp add: clink.awalk_Nil_iff)
+    then show ?case by blast
+  next
+    fix w1 w2 e es
+    assume e: "e \<in> arcs (clink H')" "arc_to_ends (with_proj (clink H')) e = (w1, w2)"
+    assume IH: "(clink'.awalk w2 es v \<Longrightarrow> \<exists>p. clink.awalk w2 p v)"
+    assume clink'_walk:"clink'.awalk w1 (e # es) v"
+    from e have disj: "w2\<rightarrow>\<^bsub>cnode H'\<^esub>w1 \<or> w1\<rightarrow>\<^bsub>cface H'\<^esub>w2"
+      unfolding clink_def reverse_def 
+      by (metis pair_union_arcs_disj arc_to_ends_pair converse_iff pair_pre_digraph.select_convs(2)
+          with_proj_simps(2) with_proj_simps(3))
+    then have "node H' w2 = w1 \<or> face H' w1 = w2"
+      by (metis Gr_eq cface_def cnode_def)
+    have "clink'.awalk w2 es v"
+      using clink'.awalk_Cons_iff clink'_walk e(2) by fastforce
+    then obtain p_ind where p_ind: "clink.awalk w2 p_ind v"
+      using IH by blast
+    consider "w1 = node H z \<and> node H' w2 = w1"
+      | "w1 \<noteq> node H z \<and> node H' w2 = w1"
+      | "w2 = face H z \<and> face H' w1 = w2"
+      | "w2 \<noteq> face H z \<and> face H' w1 = w2"
+      using \<open>(node H') \<langle>$\<rangle> w2 = w1 \<or> (face H') \<langle>$\<rangle> w1 = w2\<close> by fastforce
+    then show "\<exists>p. clink.awalk w1 p v"
+    proof cases
+      case 1
+      then have "node H w2 = z"
+        by (metis apply_skip_perm faceK skip_id skip_invariant walkup_node)
+      then show ?thesis 
+        by (metis "1" IH \<open>clink'.awalk w2 es v\<close> arc_to_ends_pair clink.awalk_ConsI clinkN 
+            hypermap.perm_node hypermap_axioms permutes_in_image with_proj_simps(2)
+            with_proj_simps(3) z_dart)
+    next
+      case 2
+      then have "node H w2 = w1"
+        by (metis DiffE Gr_eq H'_def disj apply_skip_perm cface_def cnode_def
+            pre_hypermap.select_convs(1) singletonI skip_fz skip_id skip_perm_invariant
+            walkupE_def walkup_node)
+      then have "w1\<rightarrow>\<^bsub>(cnode H)\<^sup>R\<^esub>w2"
+        unfolding cnode_def apply (auto simp add: Gr_def reverse_def Gr_eq)
+        by (metis Gr_verts UnE cface_def clink.awalk_hd_in_verts clink_def cnode_def p_ind
+            perm_node perm_on.Gr_reverse_eq_inv perm_on.intro verts_union with_proj_union)
+      then have "clink.awalk w1 (e#p_ind) v"
+        using p_ind apply auto
+        by (metis arc_to_ends_pair clink.awalk_Cons_iff clink_def e(2) pair_union_arcs_disj
+            prod.sel(1) prod.sel(2) with_proj_simps(2) with_proj_simps(3) with_proj_simps(4) 
+            with_proj_simps(5)) 
+      then show ?thesis by auto
+    next
+      case 3
+      then have "face H w1 = z"
+        by (metis apply_inj_eq_iff apply_skip_perm skip_id skip_invariant walkup_face)
+      then show ?thesis 
+        by (metis 3 IH \<open>clink'.awalk w2 es v\<close> arc_to_ends_pair clink.awalk_ConsI clinkF 
+            hypermap.perm_face hypermap_axioms permutes_in_image with_proj_simps(2)
+            with_proj_simps(3) z_dart)
+    next
+      case 4
+      then have "face H w1 = w2"
+        by (metis DiffE Gr_eq H'_def disj apply_skip_perm cface_def cnode_def
+            pre_hypermap.select_convs(1) singletonI skip_fz skip_id skip_perm_invariant
+            walkupE_def walkup_face)
+      then have "w1\<rightarrow>\<^bsub>cface H\<^esub>w2"
+        unfolding cface_def apply (auto simp add: Gr_def reverse_def Gr_eq)
+        by (metis Gr_eq Permutations.permutes_not_in cface_def cnode_def disj perm_face subset_eq 
+            walkup_darts_subset)
+      then have "clink.awalk w1 (e#p_ind) v"
+        using p_ind apply auto
+        by (metis arc_to_ends_pair clink.awalk_Cons_iff clink_def e(2) pair_union_arcs_disj
+            prod.sel(1) prod.sel(2) with_proj_simps(2) with_proj_simps(3) with_proj_simps(4) 
+            with_proj_simps(5)) 
+      then show ?thesis by auto
+    qed
+  qed
+  then obtain p where "clink.awalk u p v"
+     by blast
+  then show ?thesis
+    using clink.reachable_awalk by blast
+qed
+
+definition "skip_edge_domain \<equiv> {x. x\<rightarrow>\<^sup>*\<^bsub>cedge H\<^esub>z \<or> x\<rightarrow>\<^sup>*\<^bsub>cedge H\<^esub>node H z}"
+
+lemma eCedom: "x \<in> skip_edge_domain \<Longrightarrow> edge H x \<in> skip_edge_domain"
+  apply (auto simp: skip_edge_domain_def)
+  by (metis Gr_eq Gr_verts cedge_connect_sym cedge_def pre_digraph.converse_reachable_cases wf_cedge 
+      wf_digraph.reach_sym_arc wf_digraph_wp_iff)+
+end
+
+context not_degenerate_walkup
+begin
+
+lemma same_cskip_edge:
+  assumes "u \<notin> skip_edge_domain"
+  shows "u\<rightarrow>\<^sup>*\<^bsub>cedge H\<^esub>v \<longleftrightarrow> u\<rightarrow>\<^sup>*\<^bsub>cedge H'\<^esub>v"
+proof -
+  have "(((\<langle>$\<rangle>) (edge H')^^m) u = ((\<langle>$\<rangle>) (edge H)^^m) u)" for m
+  proof (induct m)
+    case 0 then show ?case by simp
+  next
+    case (Suc m)
+    then show ?case
+      by (smt (verit, best) assms cedge_def dart_u funpow_simp_l in_mono mem_Collect_eq nodeK
+          not_degenerate_walkup.skip_edge_invariant not_degenerate_walkup_axioms perm_edge
+          perm_on.intro perm_on.reach_iff_funpow_perm skip_edge_Perm skip_edge_domain_def
+          walkup_darts_subset walkup_edge)
+  qed
+  then show ?thesis
+    by (smt (verit, del_insts) cedge_def dart_u hypermap.perm_edge hypermap_walkupE
+        not_degenerate_walkup.walkup_darts_subset not_degenerate_walkup_axioms perm_edge
+        perm_on.intro perm_on.reach_iff_funpow_perm subsetD)
+qed
+
+lemma sub_cskip_edge: "\<not> cross_edge \<Longrightarrow> u\<rightarrow>\<^sup>*\<^bsub>cedge H\<^esub>v \<Longrightarrow> u\<rightarrow>\<^sup>*\<^bsub>cedge H'\<^esub>v"
+  sorry
+
+lemma cskip_edge_merge: 
+  assumes "\<not> cross_edge" "u \<in> skip_edge_domain"
+  shows "u\<rightarrow>\<^sup>*\<^bsub>cedge H'\<^esub>v \<longleftrightarrow> v \<in> skip_edge_domain"
+proof
+  show "v \<in> skip_edge_domain" if "u\<rightarrow>\<^sup>*\<^bsub>cedge H'\<^esub>v"
+    by (smt (verit, ccfv_SIG) hypermap.wf_cedge assms(2) that dart_u dart_v wf_digraph_wp_iff 
+    hypermap_walkupE mem_Collect_eq not_degenerate_walkup.intro not_degenerate_walkup.same_cskip_edge 
+    not_degenerate_walkup_axioms.intro skip_edge_domain_def walkup_axioms wf_cedge z_not_glink
+    wf_digraph.reachable_trans wf_digraph.connect_sym_def hypermap.cedge_connect_sym)
+  assume *: "v \<in> skip_edge_domain"
+  have "node H (face H z) \<noteq> z"
+      by (metis Gr_eq assms(1) cedge_def cross_edge_path_edge edgeK skip_edge_node skip_edge_noteq_z 
+          wf_cedge wf_digraph.reachable_adjI wf_digraph_wp_iff z_dart)
+  then have "edge H z \<noteq> z"
+      by (metis nodeK)
+  then show "u\<rightarrow>\<^sup>*\<^bsub>cedge H'\<^esub>v"
+      using * assms apply_inj_eq_iff apply_skip_perm perm.apply_perm_inverse pre_hypermap.select_convs(2) skip_edge_Perm skip_id u_noteq_z walkupE_def sorry
+qed
+
+lemma fcard_skip_edge:
+  defines "Sez \<equiv> if z \<rightarrow>\<^bsub>glink H\<^esub> z 
+                 then (if edge H z = z then 2 else 1) 
+                 else (if cross_edge then 0 else 2)"
+  shows "count_cycles_on (darts H') (edge H') + Sez = count_cycles_on (darts H) (edge H) + 1"
+  apply (auto simp: Sez_def)
+  using with_proj_simps(3) z_not_glink apply blast
+  apply (metis Gr_eq arc_in_union cedge_def glink_def with_proj_simps(3) z_dart)
+  apply (metis Gr_eq cedge_def cross_edge_def skip_edge_node skip_edge_noteq_z wf_cedge
+      wf_digraph.reachable_adjI wf_digraph_wp_iff z_dart)
+  using with_proj_simps(3) z_not_glink apply blast
+  defer
+  using with_proj_simps(3) z_not_glink apply blast
+  sorry
+
+end
+subsection \<open>Degenerate walkup\<close>
+text \<open>Degenerate case for walkup where one of the permutations is an identity on z\<close>
+
+locale degenerate_walkup = walkup +
   assumes z_glink: "z\<rightarrow>\<^bsub>glink H\<^esub> z"
 begin
 
-lemma z_dart: "z \<in> darts H"
-  by (metis z_glink Gr_eq cedge_def cface_def cnode_def glink_def pair_union_arcs_disj)
-
 lemma degenerate_euler:
-  defines "H' \<equiv> walkupE H z"
   shows "euler_lhs H - euler_lhs H' = euler_rhs H - euler_rhs H'"
 proof (cases "edge H z = z \<and> node H z = z \<and> face H z = z")
 interpret face_perm_on: finite_perm_on "face H" "darts H"
@@ -250,13 +578,13 @@ interpret edge_perm_on: finite_perm_on "edge H" "darts H"
   have "euler_rhs H' = euler_rhs H - 3"
   proof -
     have "count_cycles_on (darts H) (node H) = count_cycles_on (darts H') (node H') + 1"
-        by (metis True assms node_perm_on.cycle_count_skip_singleton finite_darts
+        by (metis True H'_def node_perm_on.cycle_count_skip_singleton finite_darts
             pre_hypermap.select_convs(1) pre_hypermap.select_convs(3) walkupE_def z_dart)
     also have "count_cycles_on (darts H) (face H) = count_cycles_on (darts H') (face H') + 1"
-        by (metis True assms face_perm_on.cycle_count_skip_singleton finite_darts
+        by (metis True H'_def face_perm_on.cycle_count_skip_singleton finite_darts
             pre_hypermap.select_convs(1) pre_hypermap.select_convs(4) walkupE_def z_dart)
     moreover have "count_cycles_on (darts H) (edge H) = count_cycles_on (darts H') (edge H') + 1"
-      by (metis True apply_skip_perm assms finite_darts glink_skip_edge perm.apply_perm_inverse
+      by (metis True apply_skip_perm H'_def finite_darts glink_skip_edge perm.apply_perm_inverse
           perm_edge perm_on.cycle_count_skip_singleton perm_on.intro pre_hypermap.select_convs(1)
           pre_hypermap.select_convs(2) walkupE_def z_glink z_dart)
     ultimately show ?thesis
@@ -264,31 +592,28 @@ interpret edge_perm_on: finite_perm_on "edge H" "darts H"
   qed
   also have "euler_lhs H' = euler_lhs H - 3"
   proof -
-    have dart_count: "card (darts H') = card (darts H) - 1"
-      by (simp add: assms node_perm_on.finite_S walkupE_def z_dart)
-    have "card (pre_digraph.sccs (glink H')) = card (pre_digraph.sccs (glink H)) - 1"
+    have "card (darts H') = card (darts H) - (1::int)" (is "?cdh' = ?cdh - 1")
+      using card_darts_walkup int_ops(6) node_perm_on.finite_S z_dart by auto
+    also have "int (card (pre_digraph.sccs (glink H'))) = int (card (pre_digraph.sccs (glink H))) - 1"
+      (is "?scch' = ?scch - 1")
       sorry
-    then have "card (darts H') + 2 * (card (pre_digraph.sccs (glink H'))) =
-             card (darts H) - 1 + 2 * (card (pre_digraph.sccs (glink H)) - 1)"
-      using dart_count by presburger
-    hence "card (darts H') + 2 * card (pre_digraph.sccs (glink H')) =
-            card (darts H) + 2 * card (pre_digraph.sccs (glink H)) - 3"
-      try0
+    then have "?scch' * (2::int) + ?cdh' = ?scch * (2::int) + ?cdh - (3::int)"
+      using calculation by fastforce
     then show ?thesis
-      using euler_lhs_def sledgehammer
-         sorry
+      unfolding euler_lhs_def by presburger
+  qed
   ultimately show ?thesis
-    by (metis diff_diff_cancel empty_iff euler_lhs_ge_3 euler_rhs_ge_3 z_dart)
+    by (metis diff_diff_cancel euler_lhs_ge_3 euler_rhs_ge_3 insert_absorb insert_not_empty z_dart)
 next
   case False
   then show ?thesis sorry
 qed
 end
 
+subsection \<open>Not degenerate walkup\<close>
 context not_degenerate_walkup begin
 
 lemma walkup_node_cycle_count:
-  defines "H' \<equiv> walkupE H z"
   shows "count_cycles_on (darts H) (node H) = count_cycles_on (darts H') (node H')"
 proof -
   interpret perm_on "(node H)" "(darts H)"
@@ -301,11 +626,10 @@ proof -
             skip_edge_id skip_edge_node z_dart)
     done
   then show ?thesis
-    by (simp add: assms walkupE_def)
+    by (simp add: H'_def walkupE_def)
 qed
 
 lemma walkup_face_cycle_count:
-  defines "H' \<equiv> walkupE H z"
   shows "count_cycles_on (darts H) (face H) = count_cycles_on (darts H') (face H')"
 proof -
   interpret perm_on "(face H)" "(darts H)"
@@ -318,29 +642,32 @@ proof -
             skip_edge_edge skip_edge_node z_dart z_not_glink)
     done
   then show ?thesis
-    by (simp add: assms walkupE_def)
+    by (simp add: H'_def walkupE_def)
 qed
 
 text \<open>cross_edge does not hold, so the edge cycles are merged and edge z is in the same edge cycle
       as node z\<close>
+
+lemma not_cross_edge_Walkup:
+  assumes "\<not> cross_edge"
+  shows "edge H z\<rightarrow>\<^sup>*\<^bsub>cedge H'\<^esub>node H (face H z)"
+  unfolding H'_def 
+  sorry
+
 lemma merge_walkup_path:
-  assumes "\<not> cross_edge H z"
-  shows "edge H z\<rightarrow>\<^sup>*\<^bsub>cedge (walkupE H z)\<^esub>node H z"
-  by (smt (z3) Gr_eq Permutations.permutes_not_in assms cedge_def cross_edge_def
-      hypermap.cedge_reachable_sym hypermap.skip_edge_permutes hypermap.wf_cedge hypermap_axioms
-      hypermap_walkupE not_degenerate_walkup.axioms(2) not_degenerate_walkup_axioms
-      not_degenerate_walkup_axioms_def pre_hypermap.select_convs(1) pre_hypermap.select_convs(2) 
-      reach_sym_arc skip_edge_Perm skip_edge_node walkupE_def wf_digraph_wp_iff)
+  assumes "\<not> cross_edge"
+  shows "edge H z\<rightarrow>\<^sup>*\<^bsub>cedge H'\<^esub>node H z"
+  by (metis Gr_eq Gr_verts H'_def assms cedge_def hypermap.cedge_connect_sym hypermap.perm_edge
+      hypermap.wf_cedge hypermap_walkupE not_cross_edge_Walkup permutes_in_image reachable_in_vertsE
+      skip_edge_Perm skip_edge_node walkup_edge wf_digraph.reach_sym_arc wf_digraph_wp_iff)
 
 lemma merge_walkup_edge_cycles:
-  assumes  "\<not> cross_edge H z"
-  defines "H' \<equiv> walkupE H z"
+  assumes  "\<not> cross_edge"
   shows "count_cycles_on (darts H) (edge H) = count_cycles_on (darts H') (edge H') + 1"
  sorry
 
 lemma not_cross_edge_euler_lhs:
-  assumes "\<not> cross_edge H z"
-  defines "H' \<equiv> walkupE H z"
+  assumes "\<not> cross_edge"
   shows "euler_rhs H = euler_rhs H' + 1"
 proof -
   have "count_cycles_on (darts H) (face H) = count_cycles_on (darts H') (face H')"
@@ -354,8 +681,7 @@ proof -
 qed
 
 lemma cross_edge_euler_rhs:
-  assumes "cross_edge H z"
-  defines "H' \<equiv> walkupE H z"
+  assumes "cross_edge"
   shows "euler_rhs H = euler_rhs H' + 3"
 proof -
   have "count_cycles_on (darts H) (face H) = count_cycles_on (darts H') (face H')"
@@ -363,31 +689,67 @@ proof -
   also have "count_cycles_on (darts H) (node H) = count_cycles_on (darts H') (node H')"
     by (simp add: assms walkup_node_cycle_count)
   moreover have "count_cycles_on (darts H) (edge H) = count_cycles_on (darts H') (edge H') + 3"
-    sorry
-  ultimately show ?thesis
-    unfolding euler_rhs_def by simp
-qed
+    oops
 
 text \<open>cross_edge does not hold, so the edge cycle is split\<close>
 lemma (in not_degenerate_walkup) cross_edge_walkup:
-  assumes "cross_edge H z"
+  assumes "cross_edge"
   shows "\<not>edge H z\<rightarrow>\<^sup>*\<^bsub>cedge (walkupE H z)\<^esub>node H (face H z)"
-  (*by (metis assms Gr_eq apply_inj_eq_iff apply_skip_perm arc_in_union cedge_def cface_def cnode_def
+   using assms Gr_eq apply_inj_eq_iff apply_skip_perm arc_in_union cedge_def cface_def cnode_def
       glink_def perm.apply_perm_inverse perm_eq_iff pre_hypermap.select_convs(2) skip_edge_Perm 
-      skip_id walkupE_def with_proj_simps(3))*)
-  sorry
-
+      skip_id walkupE_def with_proj_simps(3) sorry
+end
 
 section \<open>Jordan and Euler\<close>
-lemma le_genus_walkupE:
-  assumes "z \<in> darts H"
-  shows "genus (walkupE H z) \<le> genus H"
-  oops
+context walkup
+begin
 
-lemma Jordan_WalkupE:
-  assumes "z \<in> darts H"
-  shows "jordan H \<Longrightarrow> jordan (walkupE H z)"
-  oops
+definition "n_comp_z disc \<equiv> if z\<rightarrow>\<^bsub>glink H\<^esub>z
+                              then (if z_barb then 2 else 1)
+                              else (if disc then 0 else 1)"
+                                         
+lemma euler_lhs_walkupE: "n_comp_z disconnected * 2 + euler_lhs H' = euler_lhs H + 1"
+  apply (auto simp: n_comp_z_def)
+  using disconnected_not_glink with_proj_simps(3) apply blast
+  apply (simp add: disconnected_def walkup.z_barb_comp walkup_axioms)
+  defer
+  apply (metis Gr_eq arc_in_union cedge_def glink_def with_proj_simps(3) z_barb_z z_dart)
+  using disconnected_not_glink apply auto
+  sorry
 
+lemma euler_rhs_walkupE: "n_comp_z disconnected * 2 + euler_rhs H' = euler_rhs H + 1"
+  apply (auto simp: n_comp_z_def)
+  using disconnected_not_glink with_proj_simps(3) apply blast
+  apply (simp add: disconnected_def walkup.z_barb_comp walkup_axioms)
+  defer
+  apply (metis Gr_eq arc_in_union cedge_def glink_def with_proj_simps(3) z_barb_z z_dart)
+  using disconnected_not_glink with_proj_simps(3) apply blast
+  sorry
+
+lemma genus_walkupE_eq: "z\<rightarrow>\<^bsub>glink H\<^esub>z \<or> \<not> cross_edge \<Longrightarrow> genus H' = genus H"
+  apply auto
+  sorry
+
+lemma le_genus_walkupE: "genus H' \<le> genus H"
+proof (cases "z\<rightarrow>\<^bsub>glink H\<^esub>z \<or> \<not> cross_edge")
+  case True
+  then show ?thesis using genus_walkupE_eq by force
+next
+  case False
+  then have "\<not>z\<rightarrow>\<^bsub>glink H\<^esub>z \<and> cross_edge" by auto
+  then have "disconnected" sorry
+  then show ?thesis
+    sorry
+qed
+
+lemma planar_walkupE: "planar H \<Longrightarrow> planar H'"
+  by (metis bot.extremum_unique bot_nat_def le_genus_walkupE planar_def)
+
+lemma even_genus_walkupE: "even (genus H') \<Longrightarrow> even (genus H)"
+  sorry
+  (*by (smt (verit) euler_lhs_walkupE euler_rhs_walkupE genus_def)*)
+
+lemma Jordan_WalkupE: "jordan H \<Longrightarrow> jordan H'"
+  sorry
 end
 end
